Ltac 'expand_wf'

App/Lib/Iterator/Spec.v
@@ -6,7 +6,6 @@ Require Import He4.Language.Term.
 Section Specs.
 
 Variable step : step_relation.
-Variable class : Coq.Strings.String.string.
 Variable wf : state -> Prop.
 
 Notation "t1 '/' st1 '==>' t2 '/' st2" := (step (pair t1 st1) (pair t2 st2))
@@ -17,7 +16,6 @@ Notation "t1 '/' st1 '==>*' t2 '/' st2" := (multi step (pair t1 st1) (pair t2 st
 
 Definition off__no_side_effects : Prop :=
   forall st,
-  called_on_class class st ->
   wf st ->
     exists b st',
        texec "off" / st ==>* tbool b / st'
